dimsum/iris/spec2.v
@@ -35,9 +35,9 @@ Section spec.
   Let X := (spec_mod_lang EV _ state_interp).
   Local Canonical Structure X.
 
-  Lemma sim_gen_TVis ts k J Φ e os :
-    (∀ s, ▷ₒ?ts imodhandle (S:=m_state (spec_trans _ _)) J (Some e) (k tt, s) (λ σ', spec_state_interp state_interp σ' os ∗ WP{ts} σ'.1 @ ? os, J {{ Φ }})) -∗
-    WP{ts} (Spec.bind (TVis e) k) @ ? os, J {{ Φ }}.
+  Lemma sim_gen_TVis ts k Π Φ e os :
+    (∀ s, ▷ₒ?ts handle_cont (spec_trans _ _) ts Π (Some e) (k tt, s) (λ σ', spec_state_interp state_interp σ' os ∗ WP{ts} σ'.1 @ ? os, Π {{ Φ }})) -∗
+    WP{ts} (Spec.bind (TVis e) k) @ ? os, Π {{ Φ }}.
   Proof.
     iIntros "Hsim". rewrite unfold_bind/=. setoid_rewrite unfold_bind; simpl.
   Admitted.
@@ -48,9 +48,9 @@ Section spec.
     (* iSplit!. iIntros "Htgt". iApply "Hsim". by iApply "Htgt". *)
   (* Qed. *)
 
-  (* Lemma sim_src_TVis k J Φ e os : *)
-  (*   ▷ₒ imodhandle J (Some e) (SRC k tt @ ? os, J {{ Φ }}) -∗ *)
-  (*   SRC (Spec.bind (TVis e) k) @ ? os, J {{ Φ }}. *)
+  (* Lemma sim_src_TVis k Π Φ e os : *)
+  (*   ▷ₒ imodhandle Π (Some e) (SRC k tt @ ? os, Π {{ Φ }}) -∗ *)
+  (*   SRC (Spec.bind (TVis e) k) @ ? os, Π {{ Φ }}. *)
   (* Proof. *)
   (*   iIntros "Hsim". rewrite unfold_bind/=. setoid_rewrite unfold_bind; simpl. *)
   (* Admitted. *)
@@ -61,9 +61,9 @@ Section spec.
   (* Qed. *)
 
   (* TODO: This is missing lemmas for going from @ ? None to @ ? Some and back. *)
-  Lemma sim_gen_TGet ts k J Φ s :
-    (▷ₒ?ts WP{ts} (k s) @ s, J {{ Φ }}) -∗
-    WP{ts} (Spec.bind TGet k) @ s, J {{ Φ }}.
+  Lemma sim_gen_TGet ts k Π Φ s :
+    (▷ₒ?ts WP{ts} (k s) @ s, Π {{ Φ }}) -∗
+    WP{ts} (Spec.bind TGet k) @ s, Π {{ Φ }}.
   Proof.
     iIntros "Hsim". rewrite unfold_bind/=. setoid_rewrite unfold_bind; simpl.
   Admitted.
@@ -84,9 +84,9 @@ Section spec.
   (*   iIntros ([??] ?) "!>". simplify_eq. iSplit!. by iFrame. *)
   (* Qed. *)
 
-  Lemma sim_gen_TPut ts k J Φ s s' :
-    (▷ₒ?ts WP{ts} (k tt) @ s', J {{ Φ }}) -∗
-    WP{ts} (Spec.bind (TPut s') k) @ s, J {{ Φ }}.
+  Lemma sim_gen_TPut ts k Π Φ s s' :
+    (▷ₒ?ts WP{ts} (k tt) @ s', Π {{ Φ }}) -∗
+    WP{ts} (Spec.bind (TPut s') k) @ s, Π {{ Φ }}.
   Proof.
     iIntros "Hsim". rewrite unfold_bind/=. setoid_rewrite unfold_bind; simpl.
   Admitted.
@@ -107,20 +107,20 @@ Section spec.
   (*   iIntros ([??] ?) "!>". simplify_eq. iSplit!. by iFrame. *)
   (* Qed. *)
 
-  Lemma sim_gen_TAll {T} ts k J Φ os :
-    (∃/∀{ts} x, ▷ₒ?ts WP{ts} (k x) @ ? os, J {{ Φ }}) -∗
-    WP{ts} (Spec.bind (TAll T) k) @ ? os, J {{ Φ }}.
+  Lemma sim_gen_TAll {T} ts k Π Φ os :
+    (∃/∀{ts} x, ▷ₒ?ts WP{ts} (k x) @ ? os, Π {{ Φ }}) -∗
+    WP{ts} (Spec.bind (TAll T) k) @ ? os, Π {{ Φ }}.
   Proof.
     iIntros "Hsim". rewrite unfold_bind/=. setoid_rewrite unfold_bind; simpl.
   Admitted.
 
-  Lemma sim_tgt_TAll {T} x k J Φ os :
-    (▷ₒ TGT (k x) @ ? os, J {{ Φ }}) -∗
-    TGT (Spec.bind (TAll T) k) @ ? os, J {{ Φ }}.
+  Lemma sim_tgt_TAll {T} x k Π Φ os :
+    (▷ₒ TGT (k x) @ ? os, Π {{ Φ }}) -∗
+    TGT (Spec.bind (TAll T) k) @ ? os, Π {{ Φ }}.
   Proof. iIntros "Hsim". iApply sim_gen_TAll => /=. by iExists _. Qed.
-  Lemma sim_src_TAll {T} k J Φ os :
-    (∀ x, SRC (k x) @ ? os, J {{ Φ }}) -∗
-    SRC (Spec.bind (TAll T) k) @ ? os, J {{ Φ }}.
+  Lemma sim_src_TAll {T} k Π Φ os :
+    (∀ x, SRC (k x) @ ? os, Π {{ Φ }}) -∗
+    SRC (Spec.bind (TAll T) k) @ ? os, Π {{ Φ }}.
   Proof. iIntros "Hsim". by iApply sim_gen_TAll => /=. Qed.
 
   (* Lemma sim_src_TAll {T} k Π Φ os : *)
@@ -133,20 +133,20 @@ Section spec.
   (*   iIntros ([??] [??]) "!>". simplify_eq. iSplit!. iFrame. iApply "Hsim". *)
   (* Qed. *)
 
-  Lemma sim_gen_TExist {T} ts k J Φ os :
-    (∀/∃{ts} x, ▷ₒ?ts WP{ts} (k x) @ ? os, J {{ Φ }}) -∗
-    WP{ts} (Spec.bind (TExist T) k) @ ? os, J {{ Φ }}.
+  Lemma sim_gen_TExist {T} ts k Π Φ os :
+    (∀/∃{ts} x, ▷ₒ?ts WP{ts} (k x) @ ? os, Π {{ Φ }}) -∗
+    WP{ts} (Spec.bind (TExist T) k) @ ? os, Π {{ Φ }}.
   Proof.
     iIntros "Hsim". rewrite unfold_bind/=. setoid_rewrite unfold_bind; simpl.
   Admitted.
 
-  Lemma sim_tgt_TExist {T} k J Φ os :
-    (∀ x, ▷ₒ TGT (k x) @ ? os, J {{ Φ }}) -∗
-    TGT (Spec.bind (TExist T) k) @ ? os, J {{ Φ }}.
+  Lemma sim_tgt_TExist {T} k Π Φ os :
+    (∀ x, ▷ₒ TGT (k x) @ ? os, Π {{ Φ }}) -∗
+    TGT (Spec.bind (TExist T) k) @ ? os, Π {{ Φ }}.
   Proof. iIntros "Hsim". by iApply sim_gen_TExist => /=. Qed.
-  Lemma sim_src_TExist {T} x k J Φ os :
-    (SRC (k x) @ ? os, J {{ Φ }}) -∗
-    SRC (Spec.bind (TExist T) k) @ ? os, J {{ Φ }}.
+  Lemma sim_src_TExist {T} x k Π Φ os :
+    (SRC (k x) @ ? os, Π {{ Φ }}) -∗
+    SRC (Spec.bind (TExist T) k) @ ? os, Π {{ Φ }}.
   Proof. iIntros "Hsim". iApply sim_gen_TExist => /=. by iExists _. Qed.
 
   (* Lemma sim_tgt_TExist {T} k Π Φ os : *)
@@ -172,8 +172,8 @@ Section spec.
   (* Qed. *)
 
   (* TODO: Can these proofs be derived from the proofs before? *)
-  Lemma sim_tgt_TNb T (k : T → _) J Φ os :
-    ⊢ TGT (Spec.bind TNb k) @ ? os , J {{ Φ }}.
+  Lemma sim_tgt_TNb T (k : T → _) Π Φ os :
+    ⊢ TGT (Spec.bind TNb k) @ ? os , Π {{ Φ }}.
   Proof.
     rewrite unfold_bind/=. setoid_rewrite unfold_bind; simpl.
   Admitted.
@@ -183,8 +183,8 @@ Section spec.
     (* move => /spec_equiv_inv //= [? Heq2]. simplify_eq/=. destruct_all void. *)
   (* Qed. *)
 
-  Lemma sim_tgt_TNb_end J Φ os :
-    ⊢ TGT TNb @ ? os, J {{ Φ }}.
+  Lemma sim_tgt_TNb_end Π Φ os :
+    ⊢ TGT TNb @ ? os, Π {{ Φ }}.
   Proof.
   Admitted.
     (* iApply sim_tgt_expr_step_None. iIntros (?[??]?? Heq Hstep) "Hs". simplify_eq/=. iModIntro. *)
@@ -193,8 +193,8 @@ Section spec.
     (* move => /spec_equiv_inv //= [? Heq2]. simplify_eq/=. destruct_all void. *)
   (* Qed. *)
 
-  Lemma sim_src_TUb T (k : T → _) J Φ os :
-    ⊢ SRC (Spec.bind TUb k) @ ? os, J {{ Φ }}.
+  Lemma sim_src_TUb T (k : T → _) Π Φ os :
+    ⊢ SRC (Spec.bind TUb k) @ ? os, Π {{ Φ }}.
   Proof.
   Admitted.
     (* rewrite unfold_bind/=. setoid_rewrite unfold_bind; simpl. *)
@@ -203,8 +203,8 @@ Section spec.
     (* iIntros ([??] [??]) "!>". destruct_all void. *)
   (* Qed. *)
 
-  Lemma sim_src_TUb_end J Φ os :
-    ⊢ SRC TUb @ ? os, J {{ Φ }}.
+  Lemma sim_src_TUb_end Π Φ os :
+    ⊢ SRC TUb @ ? os, Π {{ Φ }}.
   Proof.
   Admitted.
     (* iApply sim_src_expr_step_None. iIntros (?[??]?) "?". simplify_eq/=. iModIntro. *)
@@ -212,21 +212,21 @@ Section spec.
     (* iIntros ([??] [??]) "!>". destruct_all void. *)
   (* Qed. *)
 
-  Lemma sim_gen_TAssume ts k J Φ (P : Prop) os :
-    (⌜P⌝ ∗/-∗{ts} ▷ₒ?ts WP{ts} (k tt) @ ? os, J {{ Φ }}) -∗
-    WP{ts} (Spec.bind (TAssume P) k) @ ? os, J {{ Φ }}.
+  Lemma sim_gen_TAssume ts k Π Φ (P : Prop) os :
+    (⌜P⌝ ∗/-∗{ts} ▷ₒ?ts WP{ts} (k tt) @ ? os, Π {{ Φ }}) -∗
+    WP{ts} (Spec.bind (TAssume P) k) @ ? os, Π {{ Φ }}.
   Proof.
     iIntros "Hsim". rewrite unfold_bind/=. setoid_rewrite unfold_bind; simpl.
   Admitted.
 
-  Lemma sim_tgt_TAssume k J Φ (P : Prop) os :
+  Lemma sim_tgt_TAssume k Π Φ (P : Prop) os :
     P →
-    (▷ₒ TGT (k tt) @ ? os, J {{ Φ }}) -∗
-    TGT (Spec.bind (TAssume P) k) @ ? os, J {{ Φ }}.
+    (▷ₒ TGT (k tt) @ ? os, Π {{ Φ }}) -∗
+    TGT (Spec.bind (TAssume P) k) @ ? os, Π {{ Φ }}.
   Proof. iIntros (?) "?". iApply sim_gen_TAssume. by iFrame. Qed.
-  Lemma sim_src_TAssume k J Φ (P : Prop) os :
-    (⌜P⌝ -∗ SRC (k tt) @ ? os, J {{ Φ }}) -∗
-    SRC (Spec.bind (TAssume P) k) @ ? os, J {{ Φ }}.
+  Lemma sim_src_TAssume k Π Φ (P : Prop) os :
+    (⌜P⌝ -∗ SRC (k tt) @ ? os, Π {{ Φ }}) -∗
+    SRC (Spec.bind (TAssume P) k) @ ? os, Π {{ Φ }}.
   Proof. iIntros "?". by iApply sim_gen_TAssume. Qed.
   (*   iIntros (?) "Hsim". rewrite unfold_bind/=. setoid_rewrite unfold_bind; simpl. *)
   (*   iApply sim_tgt_expr_step_None. iIntros (?[??]?? Heq Hstep) "Hs". simplify_eq/=. iModIntro. *)
@@ -247,21 +247,21 @@ Section spec.
   (*   iIntros ([??] [??]) "!>". simplify_eq. iSplit!. iFrame. by iApply "Hsim". *)
   (* Qed. *)
 
-  Lemma sim_gen_TAssert ts k J Φ (P : Prop) os :
-    (⌜P⌝ -∗/∗{ts} ▷ₒ?ts WP{ts} (k tt) @ ? os, J {{ Φ }}) -∗
-    WP{ts} (Spec.bind (TAssert P) k) @ ? os, J {{ Φ }}.
+  Lemma sim_gen_TAssert ts k Π Φ (P : Prop) os :
+    (⌜P⌝ -∗/∗{ts} ▷ₒ?ts WP{ts} (k tt) @ ? os, Π {{ Φ }}) -∗
+    WP{ts} (Spec.bind (TAssert P) k) @ ? os, Π {{ Φ }}.
   Proof.
     iIntros "Hsim". rewrite unfold_bind/=. setoid_rewrite unfold_bind; simpl.
   Admitted.
 
-  Lemma sim_tgt_TAssert k J Φ (P : Prop) os :
-    (⌜P⌝ -∗ ▷ₒ TGT (k tt) @ ? os, J {{ Φ }}) -∗
-    TGT (Spec.bind (TAssert P) k) @ ? os, J {{ Φ }}.
+  Lemma sim_tgt_TAssert k Π Φ (P : Prop) os :
+    (⌜P⌝ -∗ ▷ₒ TGT (k tt) @ ? os, Π {{ Φ }}) -∗
+    TGT (Spec.bind (TAssert P) k) @ ? os, Π {{ Φ }}.
   Proof. iIntros "?". by iApply sim_gen_TAssert. Qed.
-  Lemma sim_src_TAssert k J Φ (P : Prop) os :
+  Lemma sim_src_TAssert k Π Φ (P : Prop) os :
     P →
-    (SRC (k tt) @ ? os, J {{ Φ }}) -∗
-    SRC (Spec.bind (TAssert P) k) @ ? os, J {{ Φ }}.
+    (SRC (k tt) @ ? os, Π {{ Φ }}) -∗
+    SRC (Spec.bind (TAssert P) k) @ ? os, Π {{ Φ }}.
   Proof. iIntros (?) "?". iApply sim_gen_TAssert. by iFrame. Qed.
 
   (* Lemma sim_tgt_TAssert k Π Φ (P : Prop) os : *)
@@ -288,15 +288,15 @@ Section spec.
   (*   Unshelve. done. *)
   (* Qed. *)
 
-  Lemma sim_tgt_TAssumeOpt {T} o (x : T) k J Φ os :
+  Lemma sim_tgt_TAssumeOpt {T} o (x : T) k Π Φ os :
     o = Some x →
-    TGT k x @ ? os , J {{ Φ }} -∗
-    TGT (Spec.bind (TAssumeOpt o) k) @ ? os , J {{ Φ }}.
+    TGT k x @ ? os , Π {{ Φ }} -∗
+    TGT (Spec.bind (TAssumeOpt o) k) @ ? os , Π {{ Φ }}.
   Proof. iIntros (->) "Hsim". simpl. by rewrite unfold_bind/=. Qed.
 
-  Lemma sim_src_TAssumeOpt {T} (o : option T) k J Φ os :
-    (∀ x, ⌜o = Some x⌝ -∗ SRC k x @ ? os, J {{ Φ }}) -∗
-    SRC (Spec.bind (TAssumeOpt o) k) @ ? os, J {{ Φ }}.
+  Lemma sim_src_TAssumeOpt {T} (o : option T) k Π Φ os :
+    (∀ x, ⌜o = Some x⌝ -∗ SRC k x @ ? os, Π {{ Φ }}) -∗
+    SRC (Spec.bind (TAssumeOpt o) k) @ ? os, Π {{ Φ }}.
   Proof.
     iIntros "Hsim".
     destruct o => /=.
@@ -304,9 +304,9 @@ Section spec.
     - iApply sim_src_TUb.
   Qed.
 
-  Lemma sim_tgt_TAssertOpt {T} (o : option T) k J Φ os :
-    (∀ x, ⌜o = Some x⌝ -∗ TGT k x @ ? os, J {{ Φ }}) -∗
-    TGT (Spec.bind (TAssertOpt o) k) @ ? os, J {{ Φ }}.
+  Lemma sim_tgt_TAssertOpt {T} (o : option T) k Π Φ os :
+    (∀ x, ⌜o = Some x⌝ -∗ TGT k x @ ? os, Π {{ Φ }}) -∗
+    TGT (Spec.bind (TAssertOpt o) k) @ ? os, Π {{ Φ }}.
   Proof.
     iIntros "Hsim".
     destruct o => /=.
@@ -314,9 +314,9 @@ Section spec.
     - iApply sim_tgt_TNb.
   Qed.
 
-  Lemma sim_src_TAssertOpt {T} o (x : T) k J Φ os :
+  Lemma sim_src_TAssertOpt {T} o (x : T) k Π Φ os :
     o = Some x →
-    SRC k x @ ? os, J {{ Φ }} -∗
-    SRC (Spec.bind (TAssertOpt o) k) @ ? os, J {{ Φ }}.
+    SRC k x @ ? os, Π {{ Φ }} -∗
+    SRC (Spec.bind (TAssertOpt o) k) @ ? os, Π {{ Φ }}.
   Proof. iIntros (->) "Hsim". simpl. by rewrite unfold_bind/=. Qed.
 End spec.
